Foundation/Propositional/Kripke/Logic/KC.lean
@@ -33,33 +33,35 @@ instance [F.IsKC] : F.IsKP := ⟨by
 end Kripke
 
 
-namespace Logic.KC.Kripke
+namespace Hilbert
 
-instance sound : Sound Logic.KC FrameClass.KC :=
+namespace KC.Kripke
+
+instance sound : Sound Hilbert.KC FrameClass.KC :=
   instSound_of_validates_axioms $ by
     apply FrameClass.Validates.withAxiomEFQ;
     rintro F hF _ rfl;
     replace hF := Set.mem_setOf_eq.mp hF;
     apply validate_axiomWeakLEM_of_isPiecewiseStronglyConvergent
 
-instance sound_finite : Sound Logic.KC FrameClass.finite_KC :=
+instance sound_finite : Sound Hilbert.KC FrameClass.finite_KC :=
   instSound_of_validates_axioms $ by
     apply FrameClass.Validates.withAxiomEFQ;
     rintro F hF _ rfl;
     replace hF := Set.mem_setOf_eq.mp hF;
     apply validate_axiomWeakLEM_of_isPiecewiseStronglyConvergent
 
-instance consistent : Entailment.Consistent Logic.KC := consistent_of_sound_frameclass FrameClass.KC $ by
+instance consistent : Entailment.Consistent Hilbert.KC := consistent_of_sound_frameclass FrameClass.KC $ by
   use whitepoint;
   apply Set.mem_setOf_eq.mpr;
   infer_instance;
 
-instance canonical : Canonical Logic.KC FrameClass.KC := ⟨by
+instance canonical : Canonical Hilbert.KC FrameClass.KC := ⟨by
   apply Set.mem_setOf_eq.mpr;
   infer_instance;
 ⟩
 
-instance complete : Complete Logic.KC FrameClass.KC := inferInstance
+instance complete : Complete Hilbert.KC FrameClass.KC := inferInstance
 
 section FFP
 
@@ -67,7 +69,7 @@ open
   finestFiltrationTransitiveClosureModel
   Relation
 
-instance finite_complete : Complete (Logic.KC) FrameClass.finite_KC := ⟨by
+instance finite_complete : Complete (Hilbert.KC) FrameClass.finite_KC := ⟨by
   intro φ hφ;
   apply Kripke.complete.complete;
   rintro F F_con V r;
@@ -129,54 +131,20 @@ instance finite_complete : Complete (Logic.KC) FrameClass.finite_KC := ⟨by
 
 end FFP
 
-open Kripke
-open Entailment
-open Formula.Kripke
+end KC.Kripke
 
-lemma KC : Logic.KC = FrameClass.KC.logic := eq_Hilbert_Logic_KripkeFrameClass_Logic
-lemma finite_KC : Logic.KC = FrameClass.finite_KC.logic := eq_Hilbert_Logic_KripkeFrameClass_Logic
-
-instance : Logic.Int ⪱ Logic.KC := by
+instance : Hilbert.KP ⪱ Hilbert.KC := by
   constructor;
-  . apply Hilbert.weakerThan_of_subset_axioms $ by simp;
-  . apply Entailment.not_weakerThan_iff.mpr;
-    suffices ∃ φ, Logic.KC ⊢! φ ∧ ¬FrameClass.all ⊧ φ by simpa [Int.Kripke.Int];
-    use Axioms.WeakLEM (.atom 0);
-    constructor;
-    . exact wlem!;
-    . apply not_validOnFrameClass_of_exists_frame;
-      let F : Frame := {
-        World := Fin 3
-        Rel := λ x y => x = 0 ∨ (x = y)
-        rel_partial_order := {
-          refl := by omega;
-          trans := by omega;
-          antisymm := by omega;
-        }
-      };
-      use F;
-      constructor;
-      . tauto;
-      . apply not_imp_not.mpr $ isPiecewiseStronglyConvergent_of_validate_axiomWeakLEM;
-        by_contra hC;
-        have := @F.ps_convergent _ 0 1 2;
-        omega;
-
-@[simp]
-theorem proper_extension_of_KP : Logic.KP ⪱ Logic.KC := by
-  constructor;
-  . apply Entailment.weakerThan_iff.mpr;
-    suffices ∀ φ, FrameClass.KP ⊧ φ → FrameClass.KC ⊧ φ by simpa [KC.Kripke.KC, KP.Kripke.KP];
-    rintro φ hφ F hF;
-    apply hφ;
+  . apply weakerThan_of_subset_frameClass FrameClass.KP FrameClass.KC;
+    intro F hF;
     simp_all only [Set.mem_setOf_eq];
-    infer_instance;
+    infer_instance
   . apply Entailment.not_weakerThan_iff.mpr;
-    suffices ∃ φ, Logic.KC ⊢! φ ∧ ¬FrameClass.KP ⊧ φ by simpa [KP.Kripke.KP];
     use Axioms.WeakLEM (.atom 0);
     constructor;
     . simp;
-    . apply not_validOnFrameClass_of_exists_frame;
+    . apply Sound.not_provable_of_countermodel (𝓜 := FrameClass.KP)
+      apply not_validOnFrameClass_of_exists_frame;
       let F : Frame := {
         World := Fin 3,
         Rel := λ x y => x = 0 ∨ x = y
@@ -222,6 +190,20 @@ theorem proper_extension_of_KP : Logic.KP ⪱ Logic.KC := by
         have := @F.ps_convergent _ 0 1 2;
         omega;
 
-end Logic.KC.Kripke
+instance : Hilbert.Int ⪱ Hilbert.KC := calc
+  Hilbert.Int ⪱ Hilbert.KP := inferInstance
+  _           ⪱ Hilbert.KC := inferInstance
+
+end Hilbert
+
+
+namespace Logic
+
+lemma KC.Kripke.KC : Logic.KC = FrameClass.KC.logic := eq_Hilbert_Logic_KripkeFrameClass_Logic
+lemma KC.Kripke.finite_KC : Logic.KC = FrameClass.KC.logic := eq_Hilbert_Logic_KripkeFrameClass_Logic
+
+instance : Logic.KP ⪱ Logic.KC := inferInstance
+
+end Logic
 
 end LO.Propositional
