Foundation/Modal/Maximal/Basic.lean
@@ -60,13 +60,10 @@ end Formula
 open Entailment
 open Formula (trivTranslate verTranslate)
 
-lemma Hilbert.provable_of_classical_provable {H : Modal.Hilbert ℕ} {φ : Propositional.Formula ℕ} : (Propositional.Logic.Cl ⊢! φ) → (H.logic ⊢! φ.toModalFormula) := by
+lemma Hilbert.provable_of_classical_provable {H : Modal.Hilbert ℕ} {φ : Propositional.Formula ℕ} : Propositional.Hilbert.Cl ⊢! φ → (H.logic ⊢! φ.toModalFormula) := by
   intro h;
   induction h using Propositional.Hilbert.rec! with
-  | maxm ih =>
-    rcases (by simpa using ih) with (⟨_, rfl⟩ | ⟨_, rfl⟩);
-    . exact efq!;
-    . exact lem!;
+  | axm _ h => rcases h with (rfl | rfl) <;> simp;
   | mdp ihφψ ihφ => exact ihφψ ⨀ ihφ;
   | _ =>
     dsimp [Propositional.Formula.toModalFormula];
@@ -74,7 +71,7 @@ lemma Hilbert.provable_of_classical_provable {H : Modal.Hilbert ℕ} {φ : Propo
 
 namespace Logic.Triv
 
-lemma iff_trivTranslated : (Logic.Triv) ⊢! φ ⭤ φᵀ := by
+lemma iff_trivTranslated : Logic.Triv ⊢! φ ⭤ φᵀ := by
   induction φ with
   | hbox φ ih =>
     apply E!_intro;
@@ -83,7 +80,7 @@ lemma iff_trivTranslated : (Logic.Triv) ⊢! φ ⭤ φᵀ := by
   | himp _ _ ih₁ ih₂ => exact ECC!_of_E!_of_E! ih₁ ih₂;
   | _ => apply E!_id
 
-protected theorem iff_provable_Cl : Logic.Triv ⊢! φ ↔ Propositional.Logic.Cl ⊢! φᵀ.toPropFormula := by
+protected theorem iff_provable_Cl : Logic.Triv ⊢! φ ↔ Propositional.Hilbert.Cl ⊢! φᵀ.toPropFormula := by
   constructor;
   . intro h;
     induction h with
@@ -105,7 +102,7 @@ end Logic.Triv
 
 namespace Logic.Ver
 
-lemma iff_verTranslated : (Logic.Ver) ⊢! φ ⭤ φⱽ := by
+lemma iff_verTranslated : Logic.Ver ⊢! φ ⭤ φⱽ := by
   induction φ with
   | hbox =>
     apply E!_intro;
@@ -114,7 +111,7 @@ lemma iff_verTranslated : (Logic.Ver) ⊢! φ ⭤ φⱽ := by
   | himp _ _ ih₁ ih₂ => exact ECC!_of_E!_of_E! ih₁ ih₂;
   | _ => apply E!_id
 
-protected lemma iff_provable_Cl : (Logic.Ver) ⊢! φ ↔ Propositional.Logic.Cl ⊢! φⱽ.toPropFormula := by
+protected lemma iff_provable_Cl : Logic.Ver ⊢! φ ↔ Propositional.Hilbert.Cl ⊢! φⱽ.toPropFormula := by
   constructor;
   . intro h;
     induction h with
