Foundation/Propositional/Kripke/Hilbert.lean
@@ -7,9 +7,9 @@ open Kripke
 open Formula
 open Formula.Kripke
 
-
-lemma Logic.eq_Hilbert_Logic_KripkeFrameClass_Logic {H : Hilbert ℕ} {C : FrameClass}
-  [sound : Sound H.logic C] [complete : Complete H.logic C]
+lemma Logic.eq_Hilbert_Logic_KripkeFrameClass_Logic
+  {H : Hilbert ℕ} {C : FrameClass}
+  [sound : Sound H C] [complete : Complete H C]
   : H.logic = C.logic := by
   ext φ;
   constructor;
@@ -22,13 +22,13 @@ lemma Logic.eq_Hilbert_Logic_KripkeFrameClass_Logic {H : Hilbert ℕ} {C : Frame
 
 namespace Hilbert.Kripke
 
-variable {H : Hilbert ℕ} {Γ : Set (Formula ℕ)} {φ : Formula ℕ}
+variable {H H₁ H₂ : Hilbert ℕ} {Γ : Set (Formula ℕ)} {φ : Formula ℕ}
 
 section
 
-variable {C : Kripke.FrameClass}
+variable {C C₁ C₂ : Kripke.FrameClass}
 
-lemma soundness_of_validates_axiomInstances (hV : C.Validates H.axiomInstances) : H.logic ⊢! φ → C ⊧ φ := by
+lemma soundness_of_validates_axioms (hV : C.Validates H.axioms) : H ⊢! φ → C ⊧ φ := by
   intro hφ F hF;
   induction hφ with
   | verum => apply ValidOnFrame.top;
@@ -41,23 +41,13 @@ lemma soundness_of_validates_axiomInstances (hV : C.Validates H.axiomInstances) 
   | orIntroR => apply ValidOnFrame.orInst₂;
   | orElim => apply ValidOnFrame.orElim;
   | mdp => exact ValidOnFrame.mdp (by assumption) (by assumption);
-  | maxm hi =>
-    obtain ⟨ψ, h, ⟨s, rfl⟩⟩ := hi;
-    apply hV F hF (ψ⟦s⟧);
-    use ψ;
-    constructor
-    . assumption;
-    . use s;
+  | axm s hi =>
+    apply ValidOnFrame.subst;
+    apply hV F hF _ hi;
 
-lemma validates_axioms_of_validates_axiomInstances (hV : C.Validates H.axioms) : C.Validates H.axiomInstances := by
-  rintro F hF _ ⟨φ, hφ, ⟨s, rfl⟩⟩;
-  exact ValidOnFrame.subst $ hV F hF φ hφ;
+instance instSound_of_validates_axioms (hV : C.Validates H.axioms) : Sound H C := ⟨fun {_} => soundness_of_validates_axioms hV⟩
 
-instance instSound_of_validates_axioms (hV : C.Validates H.axioms) : Sound H.logic C := ⟨fun {_} =>
-  soundness_of_validates_axiomInstances (validates_axioms_of_validates_axiomInstances hV)
-⟩
-
-lemma consistent_of_sound_frameclass (C : FrameClass) (hC : Set.Nonempty C) [sound : Sound H.logic C] : Entailment.Consistent H.logic := by
+lemma consistent_of_sound_frameclass (C : FrameClass) (hC : Set.Nonempty C) [sound : Sound H C] : Entailment.Consistent H := by
   apply Entailment.Consistent.of_unprovable (f := ⊥);
   apply not_imp_not.mpr sound.sound;
   apply Semantics.set_models_iff.not.mpr;
@@ -72,6 +62,14 @@ lemma finite_sound_of_sound (sound : Sound H.logic C) : Sound H.logic ({ F | F �
   rintro φ hφ F ⟨hF₁, _⟩;
   exact sound.sound hφ hF₁;
 ⟩
+
+lemma weakerThan_of_subset_frameClass (C₁ C₂ : FrameClass) (hC : C₂ ⊆ C₁) [Sound H₁ C₁] [Complete H₂ C₂] : H₁ ⪯ H₂ := by
+  apply Entailment.weakerThan_iff.mpr;
+  intro φ hφ;
+  apply Complete.complete (𝓜 := C₂);
+  intro F hF;
+  apply Sound.sound (𝓢 := H₁) (𝓜 := C₁) hφ;
+  apply hC hF;
 
 end
 
